

Chain Rule Example - Jan 19, 2026

$$\sigma(x) = \frac{1}{1+e^{-x}} = \underbrace{(1+e^{-x})^{-1}}_{g(x)} \quad g(x) = 1 + (e^x)^{-1} = 1 + h(x)^{-1}$$

$$\frac{d\sigma}{dx} = \frac{d\sigma}{dg} \cdot \frac{dg}{dh} \cdot \frac{dh}{dx}$$

$$\frac{dh}{dx} = e^x, \quad \frac{dg}{dh} = 0 + (-h(x)^{-2}), \quad \frac{d\sigma}{dg} = -g(x)^{-2}$$

subbing back in:

$$\begin{aligned} \frac{d\sigma}{dx} &= -g(x)^{-2} \cdot -h(x) \cdot e^x \\ &= \cancel{(1+e^{-x})^{-2}} \cdot \cancel{(e^x)^{-1}} \cdot \cancel{e^x} \end{aligned}$$

$$= (1+e^{-x})^{-2} \cdot e^{-x} = \frac{e^{-x}}{(1+e^{-x})^2} //$$

→ commonly written as $\sigma(x)(1-\sigma(x))$

Linear Regression - Jan 21

$\frac{\partial \text{MSE}}{\partial \theta_0} = 0$ to find θ_0 that minimizes MSE

$$\frac{\partial}{\partial \theta_0} \left(\frac{1}{n} \sum_i (\underbrace{\theta_0 + \theta_1 x_i - y_i}_{g})^2 \right) \quad \frac{\partial g}{\partial \theta_0} = 1, \quad \frac{\partial g}{\partial \theta_1} = x_i$$

$$= \frac{1}{n} \sum_i 2g' \cdot \frac{\partial g}{\partial \theta_0} = \frac{2}{n} \sum_i (\theta_0 + \theta_1 x_i - y_i)$$

$$0 = \frac{2}{n} \left(\sum_i \theta_0 + \sum_i (\theta_1 x_i - y_i) \right)$$

$$\hookrightarrow \theta_0 = \frac{\sum_i y_i}{n} - \theta_1 \frac{\sum_i x_i}{n} = \mu_y - \theta_1 \mu_x //$$

$$\frac{\partial}{\partial \theta_1} = \frac{1}{n} \sum_i 2g \cdot \frac{\partial g}{\partial \theta_1} = \frac{2}{n} \left(\sum_i (\theta_0 + \theta_1 x_i - y_i) \cdot x_i \right)$$

$$0 = \theta_0 \sum_i x_i + \theta_1 \sum_i x_i^2 - \sum_i x_i y_i$$

$$= (\mu_y - \theta_1 \mu_x) \sum_i x_i + \theta_1 \sum_i x_i^2 - \sum_i x_i y_i$$

$$= \mu_y \sum_i x_i - \sum_i x_i y_i - \theta_1 (\mu_x \sum_i x_i - \sum_i x_i^2)$$

$$\therefore \theta_1 = \frac{\mu_y \sum_i x_i - \sum_i x_i y_i}{\mu_x \sum_i x_i - \sum_i x_i^2} //$$

Matrix Form

∇_{θ} : just like scalar, $\frac{d}{dx}(\vec{a} \vec{x}) = \vec{a}$, $\frac{d}{dx}(\vec{a} \vec{x}^T \vec{x})$

First, expand

$$\frac{1}{m} (\mathbf{x} \vec{\theta} - \vec{y})^T (\mathbf{x} \vec{\theta} - \vec{y})$$

$$\uparrow$$
$$(\mathbf{x} \vec{\theta})^T = \vec{\theta}^T \mathbf{x}^T$$

$$= 2 \vec{a} \vec{x},$$

etc

$$\frac{1}{m} (\vec{\theta}^T \mathbf{x}^T - \vec{y}^T) (\mathbf{x} \vec{\theta} - \vec{y}) = \underbrace{\vec{\theta}^T \mathbf{x}^T \mathbf{x} \vec{\theta}}_{\substack{\text{can group, both} \\ \text{end up as vectors}}} - \vec{\theta}^T \mathbf{x}^T \vec{y} - \vec{y}^T \mathbf{x} \vec{\theta} + \vec{y}^T \vec{y}$$

can group, both
end up as vectors

$$= \vec{\theta}^T \mathbf{x}^T \mathbf{x} \vec{\theta} - 2 \vec{\theta}^T \mathbf{x}^T \vec{y} + \cancel{\vec{y}^T \vec{y}}$$

$$\frac{\partial}{\partial \theta} = 0$$

$$\uparrow$$
$$\vec{\theta}^T \vec{\theta} = \sum_i \theta_i^2, \quad \frac{\partial}{\partial \theta} = 2 \mathbf{x}^T \mathbf{x} \vec{\theta}$$

$$\nabla_{\theta} = \frac{1}{m} (2 \mathbf{x}^T \mathbf{x} \vec{\theta} - 2 \mathbf{x}^T \vec{y}) = \frac{2 \mathbf{x}^T}{m} (\mathbf{x} \vec{\theta} - \vec{y}) //$$

The gradient to descend

↳ can set = 0 to get:

$$\vec{\theta} = (\mathbf{x}^T \mathbf{x})^{-1} (\mathbf{x}^T \vec{y}) \quad (\text{closed form solution})$$